test insert_bst2 behavior for extraction
hashtbls on the horizon?

test.c
@@ -7,5 +7,7 @@ int main() {
   printf("h=%lui\n", h);
   uint64_t s = P1_UInt32_main3 ();
   printf("s=%lui\n", s);
+  uint64_t r = P1_UInt32_main4 ();
+  printf("r=%lui\n", r);
   return 0;
 }
