P1_UInt32.fst
@@ -13,43 +13,71 @@ module I64 = FStar.Int64
 let t = NTreeC3.t
 let linked_tree = NTreeC3.linked_tree
 
+//let a = U32.t
+//let val0 = 0ul
+//let val1 = 1ul
+//let val2 = 2ul
+//let val3 = 3ul
+//let val4 = 4ul
+//let val42 = 42ul
+//let compare (x y: U32.t) : I64.t
+//  =
+//  if U32.gt x y then 1L
+//  else if U32.eq x y then 0L
+//  else -1L
+
+let a = (U32.t & U32.t)
+let val0 = 0ul, 0ul
+let val1 = 1ul, 1ul
+let val2 = 2ul, 2ul
+let val3 = 3ul, 3ul
+let val4 = 4ul, 4ul
+let val42 = 42ul, 42ul
+let compare (x y: a) : I64.t
+  =
+  let x = fst x in
+  let y = fst y in
+  if U32.gt x y then 1L
+  else if U32.eq x y then 0L
+  else -1L
+
 inline_for_extraction noextract
-let get_left = NTreeC3.get_left #U32.t
+let get_left = NTreeC3.get_left #a
 inline_for_extraction noextract
-let get_right = NTreeC3.get_right #U32.t
+let get_right = NTreeC3.get_right #a
 inline_for_extraction noextract
-let get_size = NTreeC3.get_size #U32.t
+let get_size = NTreeC3.get_size #a
 inline_for_extraction noextract
-let get_data = NTreeC3.get_data #U32.t
+let get_data = NTreeC3.get_data #a
 
 // will be useful later? if so, null or null_t?
 //inline_for_extraction noextract
 //let null = Steel.Reference.null
 inline_for_extraction noextract
-let is_null_t = NTreeC3.is_null_t #U32.t
+let is_null_t = NTreeC3.is_null_t #a
 
 inline_for_extraction noextract
-let mk_node = NTreeC3.mk_node #U32.t
+let mk_node = NTreeC3.mk_node #a
 
 (* not inlined *)
-let unpack_tree = NTreeC3.unpack_tree #U32.t
+let unpack_tree = NTreeC3.unpack_tree #a
 
 (* stdlib *)
-let create_leaf = P1.create_leaf #U32.t
-let create_tree = P1.create_tree #U32.t
-let merge_tree = P1.merge_tree #U32.t
-let sot_wds = P1.sot_wds #U32.t
-let append_left = P1.append_left #U32.t
-let append_right = P1.append_right #U32.t
-let height = P1.height #U32.t
-let member = P1.member #U32.t
-let insert_bst = P1.insert_bst #U32.t
-let rotate_left = P1.rotate_left #U32.t
-let rotate_right = P1.rotate_right #U32.t
-let rotate_right_left = P1.rotate_right_left #U32.t
-let rotate_left_right = P1.rotate_left_right #U32.t
-let is_balanced = P1.is_balanced #U32.t
-(* TODO: another failure "nth" (?) *)
+let create_leaf = P1.create_leaf #a
+let create_tree = P1.create_tree #a
+let merge_tree = P1.merge_tree #a
+let sot_wds = P1.sot_wds #a
+let append_left = P1.append_left #a
+let append_right = P1.append_right #a
+let height = P1.height #a
+let member = P1.member #a
+let insert_bst = P1.insert_bst #a
+let insert_bst2 = P1.insert_bst2 #a
+let rotate_left = P1.rotate_left #a
+let rotate_right = P1.rotate_right #a
+let rotate_right_left = P1.rotate_right_left #a
+let rotate_left_right = P1.rotate_left_right #a
+let is_balanced = P1.is_balanced #a
 (*
 let rebalance_avl = P1.rebalance_avl #U32.t
 let insert_avl = P1.insert_avl #U32.t
@@ -67,14 +95,14 @@ let one ()
   let r = malloc v in r
 *)
 
-let destruct_linked_tree_leaf (ptr: t U32.t) : Steel unit
+let destruct_linked_tree_leaf (ptr: t a) : Steel unit
   (linked_tree ptr) (fun _ -> emp)
   (requires fun _ -> is_null_t ptr)
   (ensures fun _ _ _ -> True)
   = sladmit ()
 
 //inline_for_extraction
-let rec destruct (ptr: t U32.t) : Steel unit
+let rec destruct (ptr: t a) : Steel unit
   (linked_tree ptr) (fun _ -> emp)
   (requires fun _ -> True)
   (ensures fun _ _ _ -> True)
@@ -91,6 +119,7 @@ let rec destruct (ptr: t U32.t) : Steel unit
     free ptr
   )*)
 
+
 let main ()
   : Steel U32.t
   (emp)
@@ -98,12 +127,12 @@ let main ()
   (requires fun _ -> True)
   (ensures fun _ _ _-> True)
   =
-  let ptr = create_tree 1ul in
-  let ptr = append_left ptr 0ul in
-  let b = member ptr 0ul in
-  let vr = if b then 42ul else 11ul in
+  let ptr = create_tree val1 in
+  let ptr = append_left ptr val2 in
+  let b = member ptr val1 in
+  let vr = if b then val42 else val0 in
   destruct ptr;
-  vr
+  return (fst vr)
 
 let main2 ()
   : Steel U64.t
@@ -113,18 +142,13 @@ let main2 ()
   (ensures fun _ _ _-> True)
   =
   let ptr = create_leaf () in
-  let ptr = append_right ptr 0ul in
-  let ptr = append_right ptr 1ul in
-  let ptr = append_right ptr 2ul in
+  let ptr = append_right ptr val1 in
+  let ptr = append_right ptr val2 in
+  let ptr = append_right ptr val3 in
   let h = height ptr in
   destruct ptr;
   h
 
-let compare (x y: U32.t) : I64.t
-  =
-  if U32.gt x y then 1L
-  else if U32.eq x y then 0L
-  else -1L
 
 let compare_is_cmp () : Lemma
 (
@@ -137,23 +161,42 @@ let compare_is_cmp () : Lemma
 ) = admit ()
 
 let main3 ()
-  : Steel U64.t
-  (emp)
-  (fun n -> emp)
+  : Steel U32.t
+  emp (fun r_n -> emp)
   (requires fun _ -> True)
   (ensures fun _ _ _-> True)
   =
   let ptr = create_leaf () in
-  let ptr = append_left ptr 0ul in
-  let ptr = append_right ptr 3ul in
-  let h = get () in
+  let ptr = append_left ptr val0 in
+  let ptr = append_right ptr val1 in
+  //let h = get () in
   //compare_is_cmp ();
-  assert (Trees.is_bst (P1.convert compare) (NTreeC3.v_linked_tree ptr h));
-  let ptr = insert_bst compare ptr 2ul in
-  let h = get () in
-  assert (Trees.is_bst (P1.convert compare) (NTreeC3.v_linked_tree ptr h));
+  //assert (Trees.is_bst (P1.convert compare) (NTreeC3.v_linked_tree ptr h));
+  let ptr = insert_bst compare ptr val2 in
+  //let h = get () in
+  //assert (Trees.is_bst (P1.convert compare) (NTreeC3.v_linked_tree ptr h));
   let h = sot_wds ptr in
-  let b = member ptr 2ul in
-  let vr = if b then 42UL else 11UL in
+  let b = member ptr val2 in
+  let vr = if b then val42 else val0 in
   destruct ptr;
-  vr
+  return (fst vr)
+
+let main4()
+  : Steel U32.t
+  emp (fun _ -> emp)
+  (requires fun _ -> True)
+  (ensures fun _ _ _ -> True)
+  =
+  let ptr = create_tree val3 in
+  let valn1 = 2ul, 1729ul in
+  let valn2 = 2ul, 42ul in
+  // toggling this flag allow one to check
+  // whether the r arg of insert_bst2 is taken into account
+  let f = true in
+  let ptr = insert_bst2 f compare ptr valn1 in
+  let ptr = insert_bst2 f compare ptr valn2 in
+  assert (I64.eq (compare valn1 valn2) I64.zero);
+  let b = member ptr valn2 in
+  let vr = if b then val42 else val0 in
+  destruct ptr;
+  return (fst vr)
